Checkpoint before complicating definitions more for program dependent refinement

src/SimulationLayer.v
@@ -1,4 +1,4 @@
-Require Import List.
+Require Import List CommonAutomation.
 
 Inductive Result {State T: Type} :=
 | Finished : State -> T -> @Result State T
@@ -52,94 +52,118 @@ Record LTS :=
     transition : forall T, State -> Op T -> @Result State T -> Prop;
   }.
 
-Record SelfSimulation (lts: LTS) (R: State lts -> State lts -> Prop):=
+Definition refines_to_related {T1 T2} refines_to (R: T2 -> T2 -> Prop) (st1 st2: T1) :=
+  exists (sr1 sr2: T2),
+    refines_to st1 sr1 /\
+    refines_to st2 sr2 /\
+    R sr1 sr2.
+
+Definition refines_to_valid {T1 T2} (refines_to: T1 -> T2 -> Prop) (valid2: T2 -> Prop) (st1: T1) : Prop :=
+  forall (st2: T2),
+    refines_to st1 st2 ->
+    valid2 st2.
+
+Definition compiles_to_valid {Op1 Op2: Type -> Type}
+           (valid_op2: forall T, Op2 T -> Prop)
+           (compiles_to: forall T, Op2 T -> Op1 T -> Prop)  T (o1: Op1 T) :=
+  exists o2, compiles_to T o2 o1 /\ valid_op2 T o2.
+
+
+Record SelfSimulation (lts: LTS)
+       (valid_state: State lts -> Prop)
+       (valid_op: forall T, Op lts T -> Prop)
+       (R: State lts -> State lts -> Prop) :=
   {
     self_simulation_correct:
       forall T o s1 s1' s2,
+        valid_state s1 ->
+        valid_state s2 ->
+        valid_op T o ->
         (transition lts) T s1 o s1' ->
         R s1 s2 ->
         exists s2',
           (transition lts) T s2 o s2' /\
           result_same s1' s2' /\
           R (extract_state s1') (extract_state s2') /\
-          (forall def, extract_ret def s1' = extract_ret def s2');
+          (forall def, extract_ret def s1' = extract_ret def s2') /\
+          valid_state (extract_state s1') /\
+          valid_state (extract_state s2') ;
   }.
 
-Record StrongBisimulation  (lts1 lts2 : LTS) (compile: forall T, Op lts2 T -> Op lts1 T) (refines_to: State lts1 -> State lts2 -> Prop):=
+Record StrongBisimulation
+       (lts1 lts2 : LTS)
+       (valid_state1 : State lts1 -> Prop)
+       (valid_op1: forall T, Op lts1 T -> Prop)
+       (valid_state2 : State lts2 -> Prop)
+       (valid_op2: forall T, Op lts2 T -> Prop)
+       (compiles_to: forall T, Op lts2 T -> Op lts1 T -> Prop)
+       (refines_to: State lts1 -> State lts2 -> Prop):=
   {
     strong_bisimulation_correct:
-      (forall T o2 s1 s2,
+      (forall T o1 o2 s1 s2,
+          valid_state1 s1 ->
+          valid_op1 T o1 ->
+          
+          valid_state2 s2 ->
+          valid_op2 T o2 ->
+          
           refines_to s1 s2 ->
+          compiles_to T o2 o1 ->
+          
           (forall s1',
-              (transition lts1) T s1 (compile T o2) s1' ->
+              (transition lts1) T s1 o1 s1' ->
               exists s2',
                 (transition lts2) T s2 o2 s2' /\
                 result_same s1' s2' /\
                 refines_to (extract_state s1') (extract_state s2') /\
-                (forall def, extract_ret def s1' = extract_ret def s2')) /\
+                (forall def, extract_ret def s1' = extract_ret def s2') /\
+                valid_state1 (extract_state s1') /\ valid_state2 (extract_state s2')) /\
           (forall s2',
               (transition lts2) T s2 o2 s2' ->
               exists s1',
-                (transition lts1) T s1 (compile T o2) s1' /\
+                (transition lts1) T s1 o1 s1' /\
                 result_same s1' s2' /\
                 refines_to (extract_state s1') (extract_state s2') /\
-                (forall def, extract_ret def s1' = extract_ret def s2')))
+                (forall def, extract_ret def s1' = extract_ret def s2')/\
+                valid_state1 (extract_state s1') /\ valid_state2 (extract_state s2')))
   }.
 
-
-
-Definition right_total {T1 T2: Type} (R: T1 -> T2 -> Prop) :=
-  forall t2, exists t1, R t1 t2.
-
-Definition refines_to_related {T1 T2} refines_to eqv_h (st1 st2: T1) :=
-  exists (sr1 sr2: T2),
-    refines_to st1 sr1 /\
-    refines_to st2 sr2 /\
-    eqv_h sr1 sr2.
-
-Definition deterministic_refinement {T1 T2} refines_to eqv_h :=
-  forall (s:T1) (sr1 sr2: T2),
-    refines_to s sr1 ->
-    refines_to s sr2 ->
-    eqv_h sr1 sr2.
-
-Definition transitive {T} (R: T -> T -> Prop) :=
-  forall t t' t'', R t t' -> R t' t'' -> R t t''.
-
-
-
-
-Theorem transfer_low_to_high :
-  forall low high eqv_h refines_to compile,
-    SelfSimulation low (refines_to_related refines_to eqv_h) ->
-    StrongBisimulation low high compile refines_to ->
-    right_total refines_to ->
-    deterministic_refinement refines_to eqv_h ->
-    transitive eqv_h ->
-    SelfSimulation high eqv_h.
+Theorem transfer_high_to_low :
+  forall low high eqv_h refines_to compiles_to valid_h valid_op_h,
+    SelfSimulation high
+                   valid_h
+                   valid_op_h
+                   eqv_h ->
+    StrongBisimulation low high
+                       (refines_to_valid refines_to valid_h)
+                       (compiles_to_valid valid_op_h compiles_to)
+                       valid_h
+                       valid_op_h
+                       compiles_to refines_to ->
+    SelfSimulation low
+                   (refines_to_valid refines_to valid_h)
+                   (compiles_to_valid  valid_op_h compiles_to)
+                   (refines_to_related refines_to eqv_h).
 Proof.
-  unfold right_total, refines_to_related, deterministic_refinement; intros.
+  unfold refines_to_related, compiles_to_valid; intros.
   destruct H, H0.
   rename self_simulation_correct0 into self_simulation_correct.
-  rename H1 into right_total_state.
   rename strong_bisimulation_correct0 into strong_bisimulation_correct.
   
-  eapply Build_SelfSimulation;  intros.
-  edestruct (right_total_state s1), (right_total_state s2).
-  eapply strong_bisimulation_correct in H1 as Hx; destruct Hx.
-  apply H6 in H.
-  repeat destruct H. destruct H7, H8.
+  eapply Build_SelfSimulation;  intros; cleanup.
+  eapply strong_bisimulation_correct in H3 as Hx; eauto; cleanup.
+  eapply H7 in H2; cleanup.
+  clear H7 H8.
+
+  eapply_fresh H in H3.
+  eapply_fresh H0 in H4.
+  eapply self_simulation_correct in H2; eauto; cleanup.  
   
-  eapply self_simulation_correct in H; eauto; repeat destruct H. destruct H10, H11.
-  repeat destruct H11.
-  destruct H13.
-  
-  eapply strong_bisimulation_correct in H4 as Hx; destruct Hx.
-  apply H15 in H.
-  destruct H, H, H17, H18.
+  eapply_fresh strong_bisimulation_correct in H4; eauto; cleanup.
+  apply H17 in H2; cleanup.
+  clear H15 H17.
   eexists; intuition eauto.
   do 2 (eapply result_same_transitive; eauto).
   apply result_same_symmetric; auto.
-  rewrite <- H9, H12; auto.
+  rewrite H11, H20; auto.  
 Qed.
-
