src/Layer1to2Refinement.v
@@ -1,0 +1,53 @@
+Require Import Primitives Layer1 BlockAllocator Layer2.
+
+Section Layer1to2Refinement.
+  
+  Fixpoint prog2to1 {T} (p1: Layer2.prog T) : Layer1.prog T :=
+    match p1 with
+    | Read a => read a
+    | Write a v => write a v
+    | Alloc v => alloc v
+    | Free a => free a
+    | Ret v => Layer1.Ret v
+    | Bind px py => Layer1.Bind (prog2to1 px) (fun x => prog2to1 (py x))
+    end.
+  
+  Fixpoint oracle_matches {T} (st1: Layer1.state) (o2: Layer2.oracle) (p: Layer2.prog T) :=
+    match p with
+    | Alloc v =>
+      forall o1' d1',
+        (Layer1.exec st1 (prog2to1 (Alloc v)) (Crashed (o1', d1')) ->
+         o2 = [Crash]) /\
+        (forall r, Layer1.exec st1 (prog2to1 (Alloc v)) (Finished (o1', d1') r) ->
+         match r with
+         | Some a =>
+           o2 = [BlockNum a]
+         | None =>
+           o2 = [DiskFull]
+         end)
+    | Bind p1 p2 =>
+       forall o1' d1',
+        (Layer1.exec st1 (prog2to1 p1) (Crashed (o1', d1')) ->
+         o2 = [Crash]) /\
+        (forall r o2' o2'',
+            Layer1.exec st1 (prog2to1 p1) (Finished (o1', d1') r) ->
+            oracle_matches st1 o2' p1 ->
+            oracle_matches (o1', d1') o2'' (p2 r) ->
+            o2 = o2'++o2'')
+    | _ =>
+      forall o1' d1',
+        (Layer1.exec st1 (prog2to1 p) (Crashed (o1', d1')) ->
+         o2 = [Crash]) /\
+        (forall r, Layer1.exec st1 (prog2to1 p) (Finished (o1', d1') r) ->
+         o2 = [Cont])
+    end.
+ 
+  Check oracle_matches.
+
+  Definition refines_to {T} st1 st2 (p: Layer2.prog T) :=
+    let '(o1, d1) := st1 in
+    let '(o2, d2) := st2 in
+    rep d2 d1 /\
+    oracle_matches st1 o2 p.
+
+  
