src/Layer2.v
@@ -1,84 +1,114 @@
-Require Import Primitives Simulation Confidentiality.
-Require Import SimpleDisk Omega FunctionalExtensionality.
-Require Import ProgLimited.
+Require Import Primitives Disk Simulation.
+Require Import Layer1 BlockAllocator.
+Require Import Omega FunctionalExtensionality Memx.
 Import ListNotations.
 Close Scope pred_scope.
 Set Implicit Arguments.
 
 Section Layer2.
-(*
-  Definition disk2 := @mem addr addr_dec sealed_value.
-  Definition state2 := (user * oracle * disk2 * store)%type.
-  Definition get_user (st: state2) := fst (fst (fst st)).
-  Definition get_oracle (st: state2) := snd (fst (fst st)).
-  Definition get_disk (st: state2) := snd (fst st).
-  Definition get_store (st: state2) := snd st.
-  *)
-  Inductive exec2 :
-    forall T, state -> prog_limited T -> @Result state T -> Prop :=
-  | Exec2Finished :
-      forall T (p: prog_limited T) u o d dh s o' d' dh' s' r,
-      exec_limited (u, o, d, s) p (Finished (u, o', d', s') r) ->
-      rep dh d ->
-      rep dh' d' ->
-      exec2 (u, o, dh, s) p (Finished (u, o', dh', s') r)
-  | Exec2Crashed :
-      forall T (p: prog_limited T) u o d dh s o' d' dh' s',
-      exec_limited (u, o, d, s) p (Crashed (u, o', d', s')) ->
-      rep dh d ->
-      rep dh' d' ->
-      exec2 (u, o, dh, s) p (Crashed (u, o', dh', s')).
 
-  Definition prog2_LTS := {| State:= state; Op:= prog_limited; transition := exec2 |}.
+  Inductive token:=
+  | BlockNum : addr -> token
+  | DiskFull : token
+  | Cont : token
+  | Crash : token.
 
-  (*
-  Definition state_equivalent_for u (st1 st2: state2) :=
-  let '(u1, o1, d1, s1) := st1 in
-  let '(u2, o2, d2, s2) := st2 in
-  u1 = u2 /\
-  o1 = o2 /\
-  @equivalent_for _ addr_dec _ u d1 d2 /\
-  @equivalent_for _ handle_dec _ u s1 s2.
-
-  Definition return_equivalent_for {T} u (ret1 ret2: @Result state2 T) :=
-    match ret1, ret2 with
-    |Finished st1 r1, Finished st2 r2 =>
-     state_equivalent_for u st1 st2 /\ r1 = r2
-    |Crashed st1, Crashed st2 =>
-     state_equivalent_for u st1 st2
-    |_, _ => False
-    end.
+  Definition oracle := list token.
   
-  Definition return_state_equivalent_for {T} u (ret1 ret2: @Result state2 T) :=
-    match ret1, ret2 with
-    |Finished s1' _, Finished s2' _
-    |Crashed s1', Crashed s2' =>
-     state_equivalent_for u s1' s2'
-    | _, _ => False
-    end.
-   *)
+  Definition state := (oracle * (disk value))%type.
+  Definition get_oracle (st: state) := fst st.
+  Definition get_disk (st: state) := snd st.
   
-  Definition state_noninterference {T} (p: prog_limited T) (valid: state -> Prop):=
-  forall viewer st1 st1' st2,
-    valid st1 ->
-    valid st2 ->
-    exec2 st1 p st1' ->
-    state_equivalent_for viewer st1 st2 ->
-    exists st2',
-      exec2 st2 p st2' /\
-      return_state_equivalent_for viewer st1' st2'.
+  Inductive prog : Type -> Type :=
+  | Read : addr -> prog (option value)
+  | Write : addr -> value -> prog (option unit)
+  | Alloc : value -> prog (option addr)
+  | Free : addr -> prog unit
+  | Ret : forall T, T -> prog T
+  | Bind : forall T T', prog T -> (T -> prog T') -> prog T'.
+   
+  Inductive exec :
+    forall T, state -> prog T -> @Result state T -> Prop :=
+  | ExecRead : 
+      forall st o' a,
+        let o := fst st in
+        let d := snd st in
+        o = Cont::o' ->
+        exec st (Read a) (Finished (o', d) (d a))
+             
+  | ExecWriteSucc :
+      forall st o' a v,
+        let o := fst st in
+        let d := snd st in
+        o = Cont::o' ->
+        d a <> None ->
+        exec st (Write a v) (Finished (o', (upd d a v)) (Some tt))
 
-  Definition ret_noninterference {T} (p: prog_limited T) (valid: state -> Prop) :=
-    forall st1 st1' st2,
-    valid st1 ->
-    valid st2 ->
-    exec2 st1 p st1' ->
-    state_equivalent_for (get_user st1) st1 st2 ->
-    exists st2',
-      exec2 st2 p st2' /\
-      return_equivalent_for (get_user st1) st1' st2'.
+  | ExecWriteFail :
+      forall st o' a v,
+        let o := fst st in
+        let d := snd st in
+        o = Cont::o' ->
+        d a = None ->
+        exec st (Write a v) (Finished (o', d) None)
 
-  Definition data_noninterference {T} (p: prog_limited T) (valid: state -> Prop) :=
-    state_noninterference p valid /\
-    ret_noninterference p valid.
+  | ExecAllocSucc :
+      forall st o' a v,
+        let o := fst st in
+        let d := snd st in
+        o = BlockNum a::o' ->
+        d a = None ->
+        exec st (Alloc v) (Finished (o', (upd d a v)) (Some a))
+
+  | ExecAllocFail :
+      forall st o' v,
+        let o := fst st in
+        let d := snd st in
+        o = DiskFull::o' ->
+        exec st (Alloc v) (Finished (o', d) None)
+
+  | ExecFree :
+      forall st o' a,
+        let o := fst st in
+        let d := snd st in
+        o = Cont::o' ->
+        exec st (Free a) (Finished (o', (delete d a)) tt)
+             
+  | ExecRet :
+      forall st o' T (v: T),
+        let o := fst st in
+        let d := snd st in
+        o = Cont::o' ->
+        exec st (Ret v) (Finished (o', d) v)
+
+  | ExecBind :
+      forall T T' (p1: prog T) (p2: T -> prog T')
+        st st1 r ret,
+        exec st p1 (Finished st1 r) ->
+        exec st1 (p2 r) ret ->
+        exec st (Bind p1 p2) ret
+             
+  | ExecOpCrash :
+      forall T st o' (p: prog T),
+        let o := fst st in
+        let d := snd st in
+        o = Crash::o' ->
+        (forall T1 (p1: prog T1) p2, p <> Bind p1 p2) ->
+        exec st p (Crashed (o', d))
+             
+  | ExecBindCrash :
+      forall T T' (p1: prog T) (p2: T -> prog T')
+        st st1,
+        exec st p1 (Crashed st1) ->
+        exec st (Bind p1 p2) (Crashed st1)
+
+  | ExecBindFail :
+      forall T T' (p1: prog T) (p2: T -> prog T')
+        st st1,
+        exec st p1 (Failed st1) ->
+        exec st (Bind p1 p2) (Failed st1).
+  (* TODO: add Failed cases *)
+  
 End Layer2.
+
+Notation "x <- p1 ;; p2" := (Bind p1 (fun x => p2))(right associativity, at level 60).
